theories/typing/unsafe/refcell/refmut_code.v
@@ -1,0 +1,161 @@
+From Coq.QArith Require Import Qcanon.
+From iris.proofmode Require Import tactics.
+From iris.algebra Require Import auth csum frac agree.
+From iris.base_logic Require Import big_op fractional.
+From lrust.lifetime Require Import na_borrow.
+From lrust.typing Require Import typing.
+From lrust.typing.unsafe.refcell Require Import refcell refmut.
+Set Default Proof Using "Type".
+
+Section refmut_functions.
+  Context `{typeG Σ, refcellG Σ}.
+
+  (* TODO : map, when we will have a nice story about closures. *)
+
+  (* Turning a refmut into a shared borrow. *)
+  Definition refmut_deref : val :=
+    funrec: <> ["x"] :=
+      let: "x'" := !"x" in
+      let: "r'" := !"x'" in
+      letalloc: "r" <- "r'" in
+      delete [ #1; "x"];; "return" ["r"].
+
+  Lemma refmut_deref_type ty :
+    typed_instruction_ty [] [] [] refmut_deref
+      (fn (fun '(α, β) => [☀α; ☀β; α ⊑ β])%EL
+          (fun '(α, β) => [# &shr{α}(refmut β ty)]%T)
+          (fun '(α, β) => &shr{α}ty)%T).
+  Proof.
+    apply type_fn; [apply _..|]. move=>/= [α β] ret arg. inv_vec arg=>x. simpl_subst.
+    eapply type_deref; [solve_typing..|by apply read_own_move|done|]=>x'.
+    iIntros "!# * #LFT Hna HE HL Hk HT". simpl_subst.
+    rewrite tctx_interp_cons tctx_interp_singleton !tctx_hasty_val.
+    iDestruct "HT" as "[Hx Hx']".
+    destruct x' as [[|lx'|]|]; try iDestruct "Hx'" as "[]".
+    iDestruct "Hx'" as (lv lrc) "#(Hfrac & #Hshr)".
+    rewrite {1}/elctx_interp 2!big_sepL_cons big_sepL_singleton.
+    iDestruct "HE" as "([Hα1 Hα2] & Hβ & #Hαβ)".
+    iMod (frac_bor_acc with "LFT Hfrac Hα1") as (qlx') "[H↦ Hcloseα1]". done.
+    rewrite heap_mapsto_vec_cons heap_mapsto_vec_singleton.
+    iDestruct (lft_glb_acc with "Hβ Hα2") as (qβα) "[Hα2β Hcloseβα2]".
+    wp_bind (!(LitV lx'))%E. iApply (wp_fupd_step with "[Hα2β]");
+         [done| |by iApply ("Hshr" with "[] Hα2β")|]; first done.
+    iMod "H↦" as "[H↦1 H↦2]". wp_read. iIntros "[#Hshr' Hα2β]!>". wp_let.
+    iDestruct ("Hcloseβα2" with "Hα2β") as "[Hβ Hα2]".
+    iMod ("Hcloseα1" with "[$H↦1 $H↦2]") as "Hα1".
+    iAssert (elctx_interp [☀ α; ☀ β; α ⊑ β] qE) with "[Hα1 Hα2 Hβ Hαβ]" as "HE".
+    { rewrite /elctx_interp 2!big_sepL_cons big_sepL_singleton. by iFrame. }
+    iApply (type_letalloc_1 (&shr{α}ty) _
+        [ x ◁ box (uninit 1); #lv ◁ &shr{α}ty]%TC with "LFT Hna HE HL Hk");
+      [solve_typing..| |]; first last.
+    { rewrite tctx_interp_cons tctx_interp_singleton tctx_hasty_val tctx_hasty_val' //.
+      iFrame. iApply (ty_shr_mono with "LFT [] Hshr'"). iApply lft_incl_glb; first done.
+      iApply lft_incl_refl. }
+    intros r. simpl_subst. eapply type_delete; [solve_typing..|].
+    eapply (type_jump [_]); solve_typing.
+  Qed.
+
+  (* Turning a refmut into a unique borrow. *)
+  Definition refmut_derefmut : val :=
+    funrec: <> ["x"] :=
+      let: "x'" := !"x" in
+      let: "r'" := !"x'" in
+      letalloc: "r" <- "r'" in
+      delete [ #1; "x"];; "return" ["r"].
+
+  Lemma refmut_derefmut_type ty :
+    typed_instruction_ty [] [] [] refmut_deref
+      (fn (fun '(α, β) => [☀α; ☀β; α ⊑ β])%EL
+          (fun '(α, β) => [# &uniq{α}(refmut β ty)]%T)
+          (fun '(α, β) => &uniq{α}ty)%T).
+  Proof.
+    apply type_fn; [apply _..|]. move=>/= [α β] ret arg. inv_vec arg=>x. simpl_subst.
+    eapply type_deref; [solve_typing..|by apply read_own_move|done|]=>x'.
+    iIntros "!# * #LFT Hna HE HL Hk HT". simpl_subst.
+    rewrite tctx_interp_cons tctx_interp_singleton !tctx_hasty_val.
+    iDestruct "HT" as "[Hx Hx']".
+    rewrite {1}/elctx_interp 2!big_sepL_cons big_sepL_singleton.
+    iDestruct "HE" as "(Hα & Hβ & #Hαβ)".
+    destruct x' as [[|lx'|]|]; try iDestruct "Hx'" as "[]".
+    iMod (bor_exists with "LFT Hx'") as (vl) "H". done.
+    iMod (bor_sep with "LFT H") as "[H↦ H]". done.
+    destruct vl as [|[[|lv|]|][|[[|lrc|]|][]]];
+      try by iMod (bor_persistent_tok with "LFT H Hα") as "[>[] _]".
+    iMod (bor_exists with "LFT H") as (ν) "H". done.
+    iMod (bor_exists with "LFT H") as (γ) "H". done.
+    iMod (bor_exists with "LFT H") as (δ) "H". done.
+    iMod (bor_exists with "LFT H") as (ty') "H". done.
+    iMod (bor_sep with "LFT H") as "[Hb H]". done.
+    iMod (bor_sep with "LFT H") as "[Hβδ H]". done.
+    iMod (bor_persistent_tok with "LFT Hβδ Hα") as "[#Hβδ Hα]". done.
+    rewrite (comm _ (1).[ν])%I. rewrite (assoc _ _ _ (1).[ν])%I.
+    iMod (bor_sep with "LFT H") as "[_ H]". done.
+    iMod (bor_fracture (λ q, (1 * q).[ν])%I with "LFT [H]") as "H". done.
+    { by rewrite Qp_mult_1_l. }
+    iDestruct (frac_bor_lft_incl _ _ 1 with "LFT H") as "#Hαν". iClear "H".
+    rewrite heap_mapsto_vec_cons. iMod (bor_sep with "LFT H↦") as "[H↦ _]". done.
+    iMod (bor_acc with "LFT H↦ Hα") as "[H↦ Hcloseα]". done.
+    wp_bind (!(LitV lx'))%E. iApply (wp_fupd_step with "[Hb]");
+      [done| |by iApply (bor_unnest with "LFT Hb")|]; first done.
+    wp_read. iIntros "Hb !>". wp_let.
+    iMod ("Hcloseα" with "[$H↦]") as "[_ Hα]".
+    iAssert (elctx_interp [☀ α; ☀ β; α ⊑ β] qE) with "[Hα Hβ Hαβ]" as "HE".
+    { rewrite /elctx_interp 2!big_sepL_cons big_sepL_singleton. by iFrame. }
+    iApply (type_letalloc_1 (&uniq{α}ty) _
+        [ x ◁ box (uninit 1); #lv ◁ &uniq{α}ty]%TC with "LFT Hna HE HL Hk");
+      [solve_typing..| |]; first last.
+    { rewrite tctx_interp_cons tctx_interp_singleton tctx_hasty_val tctx_hasty_val' //.
+      iFrame. iApply (bor_shorten with "[] Hb").
+      by iApply lft_incl_glb; [iApply lft_incl_glb|iApply lft_incl_refl]. }
+    intros r. simpl_subst. eapply type_delete; [solve_typing..|].
+    eapply (type_jump [_]); solve_typing.
+  Qed.
+
+  (* Dropping a refmut and set the count to 0 in the corresponding refcell. *)
+  Definition refmut_drop : val :=
+    funrec: <> ["x"] :=
+      let: "rc" := !("x" +ₗ #1) in
+      "rc" <- #0;;
+      Endlft;;
+      delete [ #2; "x"];;
+      let: "r" := new [ #0] in "return" ["r"].
+
+  Lemma refmut_drop_type ty :
+    typed_instruction_ty [] [] [] refmut_drop
+      (fn (fun α => [☀α])%EL (fun α => [# refmut α ty])  (fun α => unit)).
+  Proof.
+    apply type_fn; [apply _..|]. move=>/= α ret arg. inv_vec arg=>x. simpl_subst.
+    iIntros "!# * #LFT Hna Hα HL Hk Hx".
+    rewrite {1}/elctx_interp big_sepL_singleton tctx_interp_singleton tctx_hasty_val.
+    destruct x as [[|lx|]|]; try iDestruct "Hx" as "[]". iDestruct "Hx" as "[Hx Hx†]".
+    iDestruct "Hx" as ([|[[|lv|]|][|[[|lrc|]|][]]]) "Hx"; try iDestruct "Hx" as "[_ >[]]".
+    rewrite {1}heap_mapsto_vec_cons heap_mapsto_vec_singleton.
+    iDestruct "Hx" as "[[Hx↦1 Hx↦2] Hx]". wp_op. wp_read. wp_let.
+    iDestruct "Hx" as (ν γ β ty') "(Hb & #Hαβ & #Hinv & Hν & H◯)".
+    iMod (lft_incl_acc with "Hαβ Hα") as (qβ) "[Hβ Hcloseα]". done.
+    iMod (na_bor_acc with "LFT Hinv Hβ Hna") as "(INV & Hna & Hcloseβ)"; [done..|].
+    iDestruct "INV" as (st) "(H↦lrc & H● & INV)". wp_write.
+    iDestruct (own_valid_2 with "H● H◯") as %[[[=]| (? & [agν st'] & [=<-] & -> &
+      [[Hag Heq]|[_ Hle]%prod_included])]%option_included []]%auth_valid_discrete_2;
+      last first.
+    { by destruct (exclusive_included (Cinl (Excl ())) st'). }
+    setoid_subst. iDestruct "INV" as (ν') "(Hνν' & H† & _)".
+    iDestruct "Hνν'" as %<-%(inj to_agree)%leibniz_equiv.
+    wp_bind Endlft. iApply (wp_fupd_step with "[H† Hν]");
+      [done| |iApply ("H†" with "Hν")|]; first done.
+    wp_seq. iIntros "{Hb} Hb !>".
+    iMod ("Hcloseβ" with ">[H↦lrc H● H◯ Hb] Hna") as "[Hβ Hna]".
+    { iExists None. iFrame. iMod (own_update_2 with "H● H◯") as "$"; last done.
+      apply auth_update_dealloc. rewrite -(right_id None _ (Some _)).
+      apply op_local_update_cancellable_empty, _. }
+    iMod ("Hcloseα" with "Hβ") as "Hα". wp_seq.
+    iAssert (elctx_interp [☀ α] qE) with "[Hα]" as "HE".
+    { by rewrite /elctx_interp big_sepL_singleton. }
+    iApply (type_delete _ _ [ #lx ◁ box (uninit 2)]%TC with "LFT Hna HE HL Hk");
+      [solve_typing..| |]; first last.
+    { rewrite tctx_interp_singleton tctx_hasty_val' //. iFrame. iExists [ #lv;#lrc].
+      rewrite heap_mapsto_vec_cons heap_mapsto_vec_singleton uninit_own. iFrame. auto. }
+    eapply type_new; [solve_typing..|]=>r. simpl_subst.
+    eapply (type_jump [_]); solve_typing.
+  Qed.
+End refmut_functions.
